src/ConcurrentFS.v
@@ -155,17 +155,17 @@ Section ConcurrentFS.
   Lemma precondition_stable_rely_fwd : forall A T (spec: FsSpec A T) tid a
                                      sigma tree homedirs sigma',
       precondition_stable spec homedirs tid ->
-      fs_invariant P (Sigma.disk sigma) (Sigma.hm sigma) tree homedirs (Sigma.mem sigma) ->
+      fs_invariant P (Sigma.init_disk sigma) (Sigma.disk sigma) (Sigma.hm sigma) tree homedirs (Sigma.mem sigma) ->
       Rely G tid sigma sigma' ->
       fs_pre (spec a) tree ->
       exists tree',
-        fs_invariant P (Sigma.disk sigma') (Sigma.hm sigma') tree' homedirs (Sigma.mem sigma') /\
+        fs_invariant P (Sigma.init_disk sigma') (Sigma.disk sigma') (Sigma.hm sigma') tree' homedirs (Sigma.mem sigma') /\
         homedir_rely tid homedirs tree tree' /\
         fs_pre (spec a) tree'.
   Proof.
     unfold precondition_stable; intros.
     match goal with
-    | [ H: fs_invariant _ _ _ _ _ _,
+    | [ H: fs_invariant _ _ _ _ _ _ _,
            H': Rely _ _ _ _ |- _ ] =>
       pose proof (fs_rely_invariant H H')
     end; deex.
@@ -178,30 +178,29 @@ Section ConcurrentFS.
       cprog_spec G tid
                  (fun '(tree, homedirs) sigma =>
                     {| precondition :=
-                         fs_invariant P (Sigma.disk sigma) (Sigma.hm sigma) tree homedirs
+                         fs_invariant P (Sigma.init_disk sigma) (Sigma.disk sigma) (Sigma.hm sigma) tree homedirs
                                       (Sigma.mem sigma) /\
                          Sigma.l sigma = Free;
                        postcondition :=
                          fun sigma' '(c, mscs) =>
                            exists tree',
-                             fs_invariant P (Sigma.disk sigma') (Sigma.hm sigma') tree' homedirs
+                             fs_invariant P (Sigma.init_disk sigma') (Sigma.disk sigma') (Sigma.hm sigma') tree' homedirs
                                           (Sigma.mem sigma') /\
                              hashmap_le (Sigma.hm sigma) (Sigma.hm sigma') /\
                              Rely G tid sigma sigma' /\
                              homedir_rely tid homedirs tree tree' /\
                              (* mscs and c come from fs_invariant on sigma *)
-                             (exists vd, cache_rep (Sigma.disk sigma) c vd /\
+                             (exists d vd, cache_rep d c vd /\
                                     fs_rep P vd (Sigma.hm sigma') mscs tree) /\
-                             Sigma.l sigma' = Sigma.l sigma /\
-                             Sigma.init_disk sigma' = Sigma.disk sigma'; |})
+                             Sigma.l sigma' = Sigma.l sigma; |})
                  readCacheMem.
   Proof using Type.
     unfold readCacheMem; intros.
     step.
     destruct a as (tree & homedirs); simpl in *; intuition.
     match goal with
-    | [ H: fs_invariant _ _ _ _ _ _ |- _ ] =>
-      pose proof (fs_invariant_unfold H); repeat deex
+    | [ H: fs_invariant _ _ _ _ _ _ _ |- _ ] =>
+      pose proof (fs_invariant_unfold_exists_disk H); repeat deex
     end.
     descend; simpl in *; intuition eauto.
 
@@ -235,17 +234,15 @@ Section ConcurrentFS.
                  simpl in *; subst;
                  (intuition (try eassumption; eauto)); try congruence.
 
-  Lemma fs_rep_same_disk_incr_hashmap : forall d d' hm hm' tree homedirs h,
+  Lemma fs_rep_same_disk_incr_hashmap : forall d_i d d' hm hm' tree homedirs h,
       d' = d ->
       hashmap_le hm hm' ->
-      fs_invariant P d hm tree homedirs h ->
-      fs_invariant P d' hm' tree homedirs h.
+      fs_invariant P d_i d hm tree homedirs h ->
+      fs_invariant P d_i d' hm' tree homedirs h.
   Proof.
     unfold fs_invariant; intros.
     SepAuto.pred_apply; SepAuto.cancel; eauto.
   Qed.
-
-  Hint Resolve fs_rep_same_disk_incr_hashmap.
 
   Theorem readonly_syscall_ok : forall T (p: OptimisticProg T) A
                                   (fsspec: FsSpec A T) tid,
@@ -255,7 +252,7 @@ Section ConcurrentFS.
       cprog_spec G tid
                  (fun '(tree, homedirs, a) sigma =>
                     {| precondition :=
-                         (fs_invariant P (Sigma.disk sigma) (Sigma.hm sigma) tree homedirs)
+                         (fs_invariant P (Sigma.init_disk sigma) (Sigma.disk sigma) (Sigma.hm sigma) tree homedirs)
                            (Sigma.mem sigma) /\
                          Sigma.l sigma = Free /\
                          fs_pre (fsspec a) tree /\
@@ -263,12 +260,11 @@ Section ConcurrentFS.
                        postcondition :=
                          fun sigma' r =>
                            exists tree',
-                             (fs_invariant P (Sigma.disk sigma') (Sigma.hm sigma') tree' homedirs)
+                             (fs_invariant P (Sigma.init_disk sigma') (Sigma.disk sigma') (Sigma.hm sigma') tree' homedirs)
                                (Sigma.mem sigma') /\
                              Rely G tid sigma sigma' /\
                              homedir_rely tid homedirs tree tree' /\
                              Sigma.l sigma' = Free /\
-                             Sigma.init_disk sigma' = Sigma.disk sigma' /\
                              match r with
                              | Done v => fs_post (fsspec a) v
                              | TryAgain => True
@@ -286,10 +282,23 @@ Section ConcurrentFS.
 
     step.
     unfold translated_postcondition in *; simplify.
-    finish.
+    intuition.
+    descend; intuition eauto.
+    repeat match goal with
+           | [ H: _ = _ |- _ ] =>
+             progress rewrite H in *
+           end;
+      eauto using fs_rep_same_disk_incr_hashmap.
 
     etransitivity; eauto.
     eapply fs_rely_same_fstree; eauto.
+    repeat match goal with
+           | [ H: _ = _ |- _ ] =>
+             progress rewrite H in *
+           end;
+      eauto using fs_rep_same_disk_incr_hashmap.
+
+    congruence.
     destruct_goal_matches; intuition auto.
   Qed.
 
@@ -338,11 +347,52 @@ Section ConcurrentFS.
     eapply fs_rep_hashmap_incr; unfold fs_rep; finish.
   Qed.
 
+  Lemma fs_invariant_forward_init_disk : forall d_i d hm tree homedirs h,
+      fs_invariant P d_i d hm tree homedirs h ->
+      fs_invariant P d d hm tree homedirs h.
+  Proof.
+    unfold fs_invariant; intros.
+  (* this isn't true: the invariant might be using d_i and ignoring d; we
+      can rule this out by knowing that whenever the lock is released the disks
+      collapse; the invariant itself could state this if the lock were the
+      global state (Free | Owned tid), or maybe it can be folded into the
+      semantics *)
+  Abort.
+
+  Definition GetWriteLock_fs_ok : forall tid,
+      cprog_spec G tid
+                 (fun '(tree, homedirs) sigma =>
+                    {| precondition :=
+                         fs_invariant P (Sigma.init_disk sigma) (Sigma.disk sigma) (Sigma.hm sigma) tree homedirs
+                                      (Sigma.mem sigma) /\
+                         Sigma.l sigma = Free;
+                       postcondition :=
+                         fun sigma' _ =>
+                           exists tree',
+                             fs_invariant P (Sigma.init_disk sigma') (Sigma.disk sigma') (Sigma.hm sigma') tree' homedirs
+                                          (Sigma.mem sigma') /\
+                             Rely G tid sigma sigma' /\
+                             homedir_rely tid homedirs tree tree' /\
+                             Sigma.l sigma' = WriteLock /\
+                             Sigma.init_disk sigma' = Sigma.disk sigma' ; |})
+                 GetWriteLock.
+  Proof using Type.
+    intros.
+    step.
+    destruct a as (tree & homedirs); simpl in *; intuition.
+
+    step.
+    intuition trivial.
+    edestruct fs_rely_invariant; eauto.
+    destruct sigma'; simpl in *.
+    descend; intuition eauto.
+  Abort.
+
   Definition startLocked_ok : forall tid,
       cprog_spec G tid
                  (fun '(tree, homedirs) sigma =>
                     {| precondition :=
-                         fs_invariant P (Sigma.disk sigma) (Sigma.hm sigma) tree homedirs
+                         fs_invariant P (Sigma.init_disk sigma) (Sigma.disk sigma) (Sigma.hm sigma) tree homedirs
                                       (Sigma.mem sigma) /\
                          Sigma.l sigma = Free;
                        postcondition :=
@@ -368,10 +418,10 @@ Section ConcurrentFS.
     edestruct fs_rely_invariant; eauto.
     destruct sigma'; simpl in *.
     match goal with
-    | [ H: fs_invariant _ _ _ _ _ _ |- _ ] =>
+    | [ H: fs_invariant _ _ _ _ _ _ _ |- _ ] =>
       pose proof (fs_invariant_unfold H); repeat deex
-    end.
-    descend; simpl in *; intuition eauto.
+    end;
+      descend; simpl in *; intuition eauto.
 
     step.
     intuition auto.
@@ -379,12 +429,12 @@ Section ConcurrentFS.
 
     unfold fs_guarantee; simpl.
     descend; intuition eauto.
-    reflexivity.
+    (* reflexivity.
 
     eapply Rely_trans; eauto.
     eapply fs_rely_same_fstree; eauto.
-    eapply fs_homedir_rely; eauto.
-  Qed.
+    eapply fs_homedir_rely; eauto. *)
+  Abort.
 
   Hint Extern 1 {{ startLocked; _ }} => apply startLocked_ok : prog.
 
